src/casemate-check-rocq/src/parser.ml
@@ -30,7 +30,7 @@ let msr_sysreg = function
 let hint_kind = function
   | Atom "set_root_lock"        -> GHOST_HINT_SET_ROOT_LOCK
   | Atom "set_owner_root"       -> GHOST_HINT_SET_OWNER_ROOT
-  | Atom "release_table"        -> GHOST_HINT_RELEASE
+  | Atom "release_table"        -> GHOST_HINT_RELEASE_TABLE
   | Atom "set_pte_thread_owner" -> GHOST_HINT_SET_PTE_THREAD_OWNER
   | sexp -> of_sexp_error "bad lock hint kind" sexp
 
@@ -102,42 +102,42 @@ let transition sexp =
   let data, id, tid, tl = match sexp with
   | List (Atom "mem-write" :: id :: tid ::
         List [Atom "mem-order"; o] :: List [Atom "address"; a] :: List [Atom "value"; v] :: tl) ->
-      GSMDT_TRANS_MEM_WRITE { twd_mo = mem_write_order o; twd_phys_addr = u64 a; twd_val = u64 v },
+      CMSD_TRANS_HW_MEM_WRITE { twd_mo = mem_write_order o; twd_phys_addr = u64 a; twd_val = u64 v },
       id, tid, tl
   | List (Atom "mem-set" :: id :: tid::
         List [Atom "address"; a] :: List [Atom "size"; s] :: List [Atom "value"; v] :: tl) ->
       if u64 s <> ~$4096 then of_sexp_error "bad mem-set size" sexp else
-      GSMDT_TRANS_MEM_WRITE { twd_mo = WMO_page; twd_phys_addr = u64 a; twd_val = u64 v },
+      CMSD_TRANS_HW_MEM_WRITE { twd_mo = WMO_page; twd_phys_addr = u64 a; twd_val = u64 v },
       id, tid, tl
   | List (Atom "mem-read" :: id :: tid::
         List [Atom "address"; a] :: List [Atom "value"; v] :: tl) ->
-      GSMDT_TRANS_MEM_READ { trd_phys_addr = u64 a; trd_val = u64 v },
+      CMSD_TRANS_HW_MEM_READ { trd_phys_addr = u64 a; trd_val = u64 v },
       id, tid, tl
   | List (Atom "mem-init" :: id :: tid::
         List [Atom "address"; a] :: List [Atom "size"; s] :: tl) ->
-      GSMDT_TRANS_MEM_ZALLOC { tzd_addr = u64 a; tzd_size = u64 s },
+      CMSD_TRANS_ABS_MEM_INIT { tid_addr = u64 a; tid_size = u64 s },
       id, tid, tl
   | List (Atom "barrier" :: id :: tid :: Atom "isb" :: tl) ->
-      GSMDT_TRANS_BARRIER (Barrier_ISB ()), id, tid, tl
+      CMSD_TRANS_HW_BARRIER (Barrier_ISB ()), id, tid, tl
   | List (Atom "barrier" :: id :: tid :: Atom "dsb" :: List [Atom "kind"; kind] :: tl) ->
-      GSMDT_TRANS_BARRIER (Barrier_DSB (barrier_kind kind)), id, tid, tl
+      CMSD_TRANS_HW_BARRIER (Barrier_DSB (barrier_kind kind)), id, tid, tl
   | List (Atom "tlbi" :: id :: tid::
         Atom kind :: List [Atom "addr"; a] :: List [Atom "level"; level] :: tl) ->
-      GSMDT_TRANS_TLBI (tlbi_of kind (Some a) (Some level) sexp), id, tid, tl
+      CMSD_TRANS_HW_TLBI (tlbi_of kind (Some a) (Some level) sexp), id, tid, tl
   | List (Atom "tlbi" :: id :: tid:: Atom kind :: tl) ->
-      GSMDT_TRANS_TLBI (tlbi_of kind None None sexp), id, tid, tl
+      CMSD_TRANS_HW_TLBI (tlbi_of kind None None sexp), id, tid, tl
   | List (Atom "sysreg-write" :: id :: tid::
         List [Atom "sysreg"; sysreg] :: List [Atom "value"; v] :: tl) ->
-      GSMDT_TRANS_MSR { tmd_sysreg = msr_sysreg sysreg; tmd_val = u64 v },
+      CMSD_TRANS_HW_MSR { tmd_sysreg = msr_sysreg sysreg; tmd_val = u64 v },
       id, tid, tl
   | List (Atom "hint" :: id :: tid::
         List [Atom "kind"; kind] :: List [Atom "location"; loc] :: List [Atom "value"; v] :: tl) ->
-      GSMDT_TRANS_HINT { thd_hint_kind = hint_kind kind; thd_location = u64 loc; thd_value = u64 v },
+      CMSD_TRANS_HINT { thd_hint_kind = hint_kind kind; thd_location = u64 loc; thd_value = u64 v },
       id, tid, tl
-  | List (Atom "lock" :: id :: tid :: List [Atom "address"; a] :: tl) ->
-      GSMDT_TRANS_LOCK { tld_kind = LOCK; tld_addr = u64 a }, id, tid, tl
-  | List (Atom "unlock" :: id :: tid :: List [Atom "address"; a] :: tl) ->
-      GSMDT_TRANS_LOCK { tld_kind = UNLOCK; tld_addr = u64 a }, id, tid, tl
+  | List (Atom "lock" :: id :: tid :: List [ Atom "address"; addr ] :: tl) ->
+    (CMSD_TRANS_ABS_LOCK (u64 addr), id, tid, tl)
+  | List (Atom "unlock" :: id :: tid :: List [ Atom "address"; addr ] :: tl) ->
+    (CMSD_TRANS_ABS_UNLOCK (u64 addr), id, tid, tl)
   | sexp -> of_sexp_error "bad event" sexp
   in
   let id = match id with
@@ -152,10 +152,10 @@ let transition sexp =
     | sexp -> of_sexp_error "bad location or extra data" (List sexp)
   in
   Some {
-    gsmt_src_loc = loc;
-    gsmt_id = id;
-    gsmt_thread_identifier = tid;
-    gsmt_data = data
+    cms_src_loc = loc;
+    cms_id = id;
+    cms_thread_identifier = tid;
+    cms_data = data
   }
 
 let of_line line = Sexplib.Sexp.of_string_conv_exn line transition
