src/casemate-check-rocq/theories/main.v
@@ -5,60 +5,26 @@ Require Export model.
 Require Export pgtable.
 Require Export step.
 
-Definition step
-  (trans : ghost_simplified_model_transition) 
-  (gsm : ghost_simplified_model) : 
-  ghost_simplified_model_result :=
-  match trans.(gsmt_data) with
-  | GSMDT_TRANS_MEM_WRITE wd =>
-      step_write trans.(gsmt_thread_identifier) wd gsm
-  | GSMDT_TRANS_MEM_ZALLOC zd =>
-      step_zalloc zd gsm
-  | GSMDT_TRANS_MEM_READ rd =>
-      step_read trans.(gsmt_thread_identifier) rd gsm
-  | GSMDT_TRANS_BARRIER ( Barrier_DSB dsb_data) =>
-      step_dsb trans.(gsmt_thread_identifier) dsb_data gsm
-  | GSMDT_TRANS_BARRIER (_) =>
-      {| gsmsr_log := []; gsmsr_data := Ok _ _ gsm |}
-  | GSMDT_TRANS_TLBI tlbi_data =>
-      step_tlbi trans.(gsmt_thread_identifier) tlbi_data gsm
-  | GSMDT_TRANS_MSR msr_data =>
-      step_msr trans.(gsmt_thread_identifier) msr_data gsm
-  | GSMDT_TRANS_HINT hint_data =>
-      step_hint trans.(gsmt_thread_identifier) hint_data gsm
-  | GSMDT_TRANS_LOCK lock_data =>
-      step_lock trans.(gsmt_thread_identifier) lock_data gsm
-  end.
-
-Definition memory_init := {|
-  gsm_roots := {| pr_s1 := []; pr_s2 := []; |};
-  gsm_memory := ∅;
-  gsm_zalloc := ∅;
-  gsm_lock_addr := ∅;
-  gsm_lock_state := ∅;
-  gsm_lock_authorization := ∅;
-|}.
-
 Fixpoint steps
-  (transitions : list ghost_simplified_model_transition)
+  (transitions : list casemate_model_step)
   (logs : list log_element)
-  (gsm : ghost_simplified_model) :
-  ghost_simplified_model_result :=
+  (cms : casemate_model_state) :
+  casemate_model_result :=
   match transitions with
-    | [] => {| gsmsr_log := logs; gsmsr_data := Ok _ _ gsm; |}
+    | [] => {| cmr_log := logs; cmr_data := Ok _ _ cms; |}
     | h :: t =>
-      match step h gsm with
-        | {| gsmsr_log := logs_next; gsmsr_data := Ok _ _ st_next |} =>
+      match step h cms with
+        | {| cmr_log := logs_next; cmr_data := Ok _ _ st_next |} =>
             steps t (logs_next ++ logs) st_next
-        | {| gsmsr_log := logs_next; gsmsr_data := Error _ _ f |} =>
-            {| gsmsr_log := logs_next ++ logs; gsmsr_data := Error _ _ f |}
+        | {| cmr_log := logs_next; cmr_data := Error _ _ f |} =>
+            {| cmr_log := logs_next ++ logs; cmr_data := Error _ _ f |}
       end
   end
 .
 
 Definition run_model 
-  (transitions : list ghost_simplified_model_transition) :
-  ghost_simplified_model_result :=
-  let res := steps transitions [] memory_init in
-  res <| gsmsr_log := rev res.(gsmsr_log) |>
+  (transitions : list casemate_model_step) :
+  casemate_model_result :=
+  let res := steps transitions [] cms_init in
+  res <| cmr_log := rev res.(cmr_log) |>
 .
