src/casemate-check-rocq/theories/transitions.v
@@ -2,13 +2,10 @@ Require Import utils.
 Require Import model.
 Require Import pgtable.
 
-(* Import bv64. *)
-
 (* Inductive SecurityState := SS_NonSecure | SS_Root | SS_Realm | SS_Secure. *)
 Inductive Regime := Regime_EL3 | Regime_EL30 | Regime_EL2 | Regime_EL20 | Regime_EL10.
 Inductive Shareability := Shareability_NSH | Shareability_ISH | Shareability_OSH.
 
-(***************************************)
 (* TLBI *)
 Inductive TLBIOp :=
   | TLBIOp_DALL
@@ -139,16 +136,17 @@ Inductive MBReqDomain :=
   | MBReqTypes_All
 . *)
 
-Record DxB  := {
+Record DxB := {
   DxB_domain : MBReqDomain;
   (* DxB_types : MBReqTypes; *)
   (* DxB_nXS : bool; *)
 }.
 
-Inductive Barrier  :=
+Inductive Barrier :=
   | Barrier_DSB : DxB -> Barrier
   | Barrier_DMB : DxB -> Barrier
   | Barrier_ISB : unit -> Barrier
+  (* Speculative barriers *)
   | Barrier_SSBB : unit -> Barrier
   | Barrier_PSSBB : unit -> Barrier
   | Barrier_SB : unit -> Barrier
@@ -160,11 +158,6 @@ Inductive write_memory_order :=
   | WMO_page
   | WMO_release
 .
-
-Record trans_zalloc_data := {
-    tzd_addr : phys_addr_t;
-    tzd_size : u64;
-}.
 
 Record tlbi_op_method_by_address_space_id_data := {
   tombas_asid_or_vmid : u64;
@@ -178,7 +171,7 @@ Inductive ghost_sysreg_kind :=
 Inductive ghost_hint_kind :=
   | GHOST_HINT_SET_ROOT_LOCK
   | GHOST_HINT_SET_OWNER_ROOT
-  | GHOST_HINT_RELEASE
+  | GHOST_HINT_RELEASE_TABLE
   | GHOST_HINT_SET_PTE_THREAD_OWNER
 .
 
@@ -199,6 +192,17 @@ Record trans_read_data := {
   trd_val : u64;
 }.
 
+Record trans_init_data := {
+    tid_addr : phys_addr_t;
+    tid_size : u64;
+}.
+
+Record trans_memset_data := {
+  tmd_addr : phys_addr_t;
+  tmd_size : u64;
+  tmd_value : u64;
+}.
+
 Record trans_msr_data := {
   tmd_sysreg : ghost_sysreg_kind;
   tmd_val : u64;
@@ -207,51 +211,50 @@ Record trans_msr_data := {
 Record trans_hint_data := {
   thd_hint_kind : ghost_hint_kind;
   thd_location : phys_addr_t;
-  thd_value : owner_t;
+  thd_value : sm_owner_t;
 }.
 
-Inductive lock_kind :=
-  | LOCK
-  | UNLOCK
-.
-
 Record trans_lock_data := {
-  tld_kind : lock_kind;
   tld_addr : phys_addr_t;
 }.
 
-Inductive ghost_simplified_model_transition_data :=
-  | GSMDT_TRANS_MEM_WRITE (write_data : trans_write_data)
-  | GSMDT_TRANS_MEM_ZALLOC (zalloc_data : trans_zalloc_data)
-  | GSMDT_TRANS_MEM_READ (read_data : trans_read_data)
-  | GSMDT_TRANS_BARRIER (dsb_data : Barrier)
-  | GSMDT_TRANS_TLBI (tlbi_data : TLBI)
-  | GSMDT_TRANS_MSR (msr_data : trans_msr_data)
-  | GSMDT_TRANS_HINT (hint_data : trans_hint_data)
-  | GSMDT_TRANS_LOCK (lock_data : trans_lock_data)
+Inductive casemate_model_step_data :=
+  (* HW_step *)
+  | CMSD_TRANS_HW_MEM_WRITE (write_data : trans_write_data)
+  | CMSD_TRANS_HW_MEM_READ (read_data : trans_read_data)
+  | CMSD_TRANS_HW_BARRIER (dsb_data : Barrier)
+  | CMSD_TRANS_HW_TLBI (tlbi_data : TLBI)
+  | CMSD_TRANS_HW_MSR (msr_data : trans_msr_data)
+  (* ABS_step *)
+  | CMSD_TRANS_ABS_MEM_INIT (init_data : trans_init_data)
+  | CMSD_TRANS_ABS_MEMSET (memset_data : trans_memset_data)
+  | CMSD_TRANS_ABS_LOCK (lock_data : trans_lock_data)
+  | CMSD_TRANS_ABS_UNLOCK (unlock_data : trans_lock_data)
+  (* HINT_step *)
+  | CMSD_TRANS_HINT (hint_data : trans_hint_data)
 .
 
-Record ghost_simplified_model_transition := {
-  gsmt_src_loc : option src_loc;
-  gsmt_thread_identifier : thread_identifier;
-  gsmt_data : ghost_simplified_model_transition_data;
-  gsmt_id : nat;
+Record casemate_model_step := {
+  cms_src_loc : option src_loc;
+  cms_thread_identifier : thread_identifier;
+  cms_data : casemate_model_step_data;
+  cms_id : nat;
 }.
 
 (******************************************************************************************)
 (*                             Code for write                                             *)
 (******************************************************************************************)
 (* Visiting a page table fails with this visitor iff the visited part has an uninitialized or invalid unclean entry *)
-Definition clean_reachable_cb (ctx : page_table_context) : ghost_simplified_model_result :=
+Definition clean_reachable_cb (ctx : pgtable_traverse_context) : casemate_model_result :=
   match ctx.(ptc_loc) with
-    | None => Merror (GSME_uninitialised "clean_reachable" ctx.(ptc_addr))
+    | None => Merror (CME_uninitialised "clean_reachable" ctx.(ptc_addr))
     | Some location =>
       match location.(sl_pte) with
         | None => Mreturn ctx.(ptc_state)
         | Some descriptor =>
-          match descriptor.(ged_state) with
+          match descriptor.(eed_state) with
             | SPS_STATE_PTE_INVALID_UNCLEAN _ =>
-              Merror (GSME_unclean_child ctx.(ptc_addr))
+              Merror (CME_unclean_child ctx.(ptc_addr))
             | _ => Mreturn ctx.(ptc_state)
           end
       end
@@ -260,17 +263,17 @@ Definition clean_reachable_cb (ctx : page_table_context) : ghost_simplified_mode
 
 Definition clean_reachable
   (map : table_data_t)
-  (descriptor : ghost_exploded_descriptor)
-  (gsm : ghost_simplified_model):
-  ghost_simplified_model_result :=
+  (descriptor : entry_exploded_descriptor)
+  (cms : casemate_model_state):
+  casemate_model_result :=
   traverse_pgt_from
-    descriptor.(ged_owner)
+    descriptor.(eed_owner)
     map.(next_level_table_addr)
-    descriptor.(ged_ia_region).(range_start)
-    (next_level descriptor.(ged_level))
-    descriptor.(ged_stage)
+    descriptor.(eed_ia_region).(range_start)
+    (next_level descriptor.(eed_level))
+    descriptor.(eed_stage)
     clean_reachable_cb
-    gsm
+    cms
 .
 
 Definition step_write_table_mark_children
@@ -278,30 +281,30 @@ Definition step_write_table_mark_children
   (wmo : write_memory_order)
   (loc : sm_location)
   (val : u64)
-  (descriptor : ghost_exploded_descriptor)
-  (visitor_cb : page_table_context -> ghost_simplified_model_result)
-  (gsm : ghost_simplified_model) :
-  ghost_simplified_model_result :=
+  (descriptor : entry_exploded_descriptor)
+  (visitor_cb : pgtable_traverse_context -> casemate_model_result)
+  (cms : casemate_model_state) :
+  casemate_model_result :=
   if is_desc_valid val then
     (* Tests if the page table is well formed *)
-    match descriptor.(ged_pte_kind) with
+    match descriptor.(eed_pte_kind) with
       | PTER_PTE_KIND_TABLE map =>
-        let st := clean_reachable map descriptor gsm in
+        let st := clean_reachable map descriptor cms in
         let st := Mlog
           (Log "BBM: invalid clean->valid"%string (phys_addr_val loc.(sl_phys_addr))) st in
         Mupdate_state (traverse_pgt_from 
-                          descriptor.(ged_owner) 
+                          descriptor.(eed_owner) 
                           map.(next_level_table_addr)
-                          descriptor.(ged_ia_region).(range_start)
-                          (next_level descriptor.(ged_level))
-                          descriptor.(ged_stage)
+                          descriptor.(eed_ia_region).(range_start)
+                          (next_level descriptor.(eed_level))
+                          descriptor.(eed_stage)
                           visitor_cb) st
       | _ => Mlog
-            (Log "BBM: invalid clean->valid"%string (phys_addr_val loc.(sl_phys_addr))) (Mreturn gsm)
+            (Log "BBM: invalid clean->valid"%string (phys_addr_val loc.(sl_phys_addr))) (Mreturn cms)
     end
   else
     (* if the descriptor is invalid, do nothing *)
-    Mreturn gsm
+    Mreturn cms
 .
 
 Definition step_write_on_invalid
@@ -309,22 +312,22 @@ Definition step_write_on_invalid
   (wmo : write_memory_order)
   (loc : sm_location)
   (val : u64)
-  (gsm : ghost_simplified_model) :
-  ghost_simplified_model_result :=
+  (cms : casemate_model_state) :
+  casemate_model_result :=
   (* If the location is a PTE table, tests if its children are clean *)
   match loc.(sl_pte) with
     | None => (* This should not happen because if we write on invalid, we write on PTE *)
-      Merror (GSME_internal_error IET_unexpected_none)
+      Merror (CME_internal_error IET_unexpected_none)
     | Some descriptor =>
       let descriptor := deconstruct_pte 
           tid 
-          descriptor.(ged_ia_region).(range_start) 
-          val descriptor.(ged_level) 
-          descriptor.(ged_owner) 
-          descriptor.(ged_stage) in
+          descriptor.(eed_ia_region).(range_start) 
+          val descriptor.(eed_level) 
+          descriptor.(eed_owner) 
+          descriptor.(eed_stage) in
       let new_loc := loc <| sl_val := val |> <| sl_pte := Some descriptor |> in
-      let new_gsm := gsm <| gsm_memory := <[ loc.(sl_phys_addr) := new_loc ]> gsm.(gsm_memory) |> in
-      step_write_table_mark_children tid wmo loc val descriptor (mark_cb tid) new_gsm
+      let new_cms := cms <| cms_memory := <[ loc.(sl_phys_addr) := new_loc ]> cms.(cms_memory) |> in
+      step_write_table_mark_children tid wmo loc val descriptor (mark_cb tid) new_cms
     end
 .
 
@@ -333,13 +336,13 @@ Definition step_write_on_invalid_unclean
   (wmo : write_memory_order)
   (loc : sm_location)
   (val : u64)
-  (gsm : ghost_simplified_model) :
-  ghost_simplified_model_result :=
+  (cms : casemate_model_state) :
+  casemate_model_result :=
   (* Only invalid descriptor are allowed *)
   if is_desc_valid val then
-    (Merror (GSME_bbm_violation VT_valid_on_invalid_unclean loc.(sl_phys_addr)))
+    (Merror (CME_bbm_violation VT_valid_on_invalid_unclean loc.(sl_phys_addr)))
   else
-    Mreturn (gsm <|gsm_memory := <[loc.(sl_phys_addr) := loc <|sl_val := val|> ]> gsm.(gsm_memory) |>)
+    Mreturn (cms <|cms_memory := <[loc.(sl_phys_addr) := loc <|sl_val := val|> ]> cms.(cms_memory) |>)
 .
 
 Definition is_only_update_to_sw_bit (old new : u64) : bool :=
@@ -354,8 +357,8 @@ Definition require_bbm
   match loc.(sl_pte) with
     | None => None (* PTE cannot be valid if it is not a PTE *)
     | Some old_descriptor =>
-      let new_descriptor := deconstruct_pte tid old_descriptor.(ged_ia_region).(range_start) val old_descriptor.(ged_level) old_descriptor.(ged_owner) old_descriptor.(ged_stage) in
-      match old_descriptor.(ged_pte_kind), new_descriptor.(ged_pte_kind) with
+      let new_descriptor := deconstruct_pte tid old_descriptor.(eed_ia_region).(range_start) val old_descriptor.(eed_level) old_descriptor.(eed_owner) old_descriptor.(eed_stage) in
+      match old_descriptor.(eed_pte_kind), new_descriptor.(eed_pte_kind) with
         | PTER_PTE_KIND_INVALID, _ | _, PTER_PTE_KIND_INVALID => Some false
         | PTER_PTE_KIND_TABLE _, _ | _, PTER_PTE_KIND_TABLE _ => Some true
         | PTER_PTE_KIND_MAP r1, PTER_PTE_KIND_MAP r2 =>
@@ -372,23 +375,23 @@ Definition step_write_valid_on_valid
   (wmo : write_memory_order)
   (loc : sm_location)
   (val : u64)
-  (gsm : ghost_simplified_model) :
-  ghost_simplified_model_result :=
+  (cms : casemate_model_state) :
+  casemate_model_result :=
   match require_bbm tid loc val with (* If no change in memory: no problem*)
-    | None => Merror (GSME_internal_error IET_unexpected_none)
+    | None => Merror (CME_internal_error IET_unexpected_none)
     | Some false =>
         (* if the location des not require BBM, then we can update the value and the descriptor *)
         match loc.(sl_pte) with
           | None => (* This does not make sense because function is called on a pgt *)
-            Merror (GSME_internal_error IET_unexpected_none)
+            Merror (CME_internal_error IET_unexpected_none)
           | Some pte =>
-            let new_pte := deconstruct_pte tid pte.(ged_ia_region).(range_start) val pte.(ged_level) pte.(ged_owner) pte.(ged_stage) in
+            let new_pte := deconstruct_pte tid pte.(eed_ia_region).(range_start) val pte.(eed_level) pte.(eed_owner) pte.(eed_stage) in
             let loc := loc <| sl_val := val |> <| sl_pte := Some new_pte |> in
-            Mreturn (insert_location loc gsm)
+            Mreturn (insert_location loc cms)
         end
     | Some true =>
       (* Changing the descriptor is illegal *)
-      Merror (GSME_bbm_violation VT_valid_on_valid loc.(sl_phys_addr))
+      Merror (CME_bbm_violation VT_valid_on_valid loc.(sl_phys_addr))
   end
 .
 
@@ -397,24 +400,24 @@ Definition step_write_invalid_on_valid
   (wmo : write_memory_order)
   (loc : sm_location)
   (val : u64)
-  (gsm : ghost_simplified_model) :
-  ghost_simplified_model_result :=
+  (cms : casemate_model_state) :
+  casemate_model_result :=
   (* Invalidation of pgt: changing the state to invalid unclean unguarded *)
   let old := loc.(sl_val) in
   match loc.(sl_pte) with
   | None => (* This does not make sense because function is called on a pgt *)
-      Merror (GSME_internal_error IET_unexpected_none)
+      Merror (CME_internal_error IET_unexpected_none)
   | Some descriptor =>
-    let new_desc := descriptor <| ged_state := (SPS_STATE_PTE_INVALID_UNCLEAN {| ai_invalidator_tid := tid; ai_old_valid_desc :=  old; ai_lis := LIS_unguarded; |}) |> in
-    let gsm := (gsm <| gsm_memory := (<[ loc.(sl_phys_addr) := loc <|sl_pte := Some (new_desc)|> <| sl_val := val |> ]> gsm.(gsm_memory))|> ) in
+    let new_desc := descriptor <| eed_state := (SPS_STATE_PTE_INVALID_UNCLEAN {| ai_invalidator_tid := tid; ai_old_valid_desc :=  old; ai_lis := LIS_unguarded; |}) |> in
+    let cms := (cms <| cms_memory := (<[ loc.(sl_phys_addr) := loc <|sl_pte := Some (new_desc)|> <| sl_val := val |> ]> cms.(cms_memory))|> ) in
     Mlog (Log "BBM: valid->invalid_unclean"%string (phys_addr_val loc.(sl_phys_addr)))
-    match descriptor.(ged_pte_kind) with
+    match descriptor.(eed_pte_kind) with
     | PTER_PTE_KIND_TABLE map =>
-      let res := clean_reachable map descriptor gsm in
+      let res := clean_reachable map descriptor cms in
       let res := Mlog (Log "invalidating a table descriptor"%string (phys_addr_val loc.(sl_phys_addr))) res in
       (* If it is well formed, mark its children as page tables, otherwise, return the same error *)
       Mupdate_state (step_write_table_mark_children tid wmo loc val descriptor (mark_not_writable_cb tid)) res
-    | _ => Mreturn gsm
+    | _ => Mreturn cms
     end
   end
 .
@@ -424,12 +427,12 @@ Definition step_write_on_valid
   (wmo : write_memory_order)
   (loc : sm_location)
   (val : u64)
-  (gsm : ghost_simplified_model) :
-  ghost_simplified_model_result :=
+  (cms : casemate_model_state) :
+  casemate_model_result :=
   if is_desc_valid val
-    then step_write_valid_on_valid tid wmo loc val gsm
+    then step_write_valid_on_valid tid wmo loc val cms
   else
-    step_write_invalid_on_valid tid wmo loc val gsm
+    step_write_invalid_on_valid tid wmo loc val cms
 .
 
 Definition is_valid_state (st: sm_pte_state) : bool :=
@@ -444,32 +447,32 @@ Definition drop_write_authorisation_of_lock
   (addr : phys_addr_t)
   (wmo : write_memory_order)
   (descriptor : u64)
-  (pte : ghost_exploded_descriptor)
-  (gsm : ghost_simplified_model) :
-  ghost_simplified_model_result :=
-  match get_lock_of_owner pte.(ged_owner) gsm with
-  | None => Mreturn gsm
+  (pte : entry_exploded_descriptor)
+  (cms : casemate_model_state) :
+  casemate_model_result :=
+  match get_lock_of_owner pte.(eed_owner) cms with
+  | None => Mreturn cms
   | Some addr_lock =>
-    match lookup addr_lock gsm.(gsm_lock_state) with
+    match lookup addr_lock cms.(cms_lock_state) with
     | Some lock_owner =>
       if bool_decide (lock_owner = cpu) then
         match wmo with
         | WMO_page | WMO_plain => (* check that the write is authorized, and then drop the authorization *)
-          match lookup addr_lock gsm.(gsm_lock_authorization) with
-          | None => Merror (GSME_internal_error IET_no_write_authorization)
-          | Some write_authorized => Mreturn (gsm <| gsm_lock_authorization := insert addr_lock write_unauthorized gsm.(gsm_lock_authorization)|>)
+          match lookup addr_lock cms.(cms_lock_authorization) with
+          | None => Merror (CME_internal_error IET_no_write_authorization)
+          | Some write_authorized => Mreturn (cms <| cms_lock_authorization := insert addr_lock write_unauthorized cms.(cms_lock_authorization)|>)
           | Some write_unauthorized =>
-            if (is_desc_valid descriptor) || is_valid_state pte.(ged_state) then
-              Merror (GSME_write_without_authorization addr)
+            if (is_desc_valid descriptor) || is_valid_state pte.(eed_state) then
+              Merror (CME_write_without_authorization addr)
             else
-              Mreturn (gsm <| gsm_lock_authorization := insert addr_lock write_unauthorized gsm.(gsm_lock_authorization)|>)
+              Mreturn (cms <| cms_lock_authorization := insert addr_lock write_unauthorized cms.(cms_lock_authorization)|>)
           end
         | WMO_release => (* drop the authorization*)
-          Mreturn (gsm <| gsm_lock_authorization := insert addr_lock write_unauthorized gsm.(gsm_lock_authorization)|>)
+          Mreturn (cms <| cms_lock_authorization := insert addr_lock write_unauthorized cms.(cms_lock_authorization)|>)
         end
       else
-        Merror (GSME_transition_without_lock addr)
-    | None => Merror (GSME_transition_without_lock addr)
+        Merror (CME_transition_without_lock addr)
+    | None => Merror (CME_transition_without_lock addr)
     end
   end
 .
@@ -477,24 +480,24 @@ Definition drop_write_authorisation_of_lock
 Definition drop_write_authorisation
   (tid : thread_identifier)
   (wd : trans_write_data)
-  (gsm : ghost_simplified_model) :
-  ghost_simplified_model_result :=
+  (cms : casemate_model_state) :
+  casemate_model_result :=
   let wmo := wd.(twd_mo) in
   let val := wd.(twd_val) in
   let addr := wd.(twd_phys_addr) in
   if negb ((bv_and_64 (phys_addr_val addr) b7) b=? b0)
-    then Merror GSME_unaligned_write 
+    then Merror CME_unaligned_write 
   else
-    match gsm !! addr with
-    | None => Mreturn gsm
+    match cms !! addr with
+    | None => Mreturn cms
     | Some location =>
         match location.(sl_pte) with
-        | None => Mreturn gsm
+        | None => Mreturn cms
         | Some pte =>
-          if is_loc_thread_owned tid location gsm then
-            Mreturn gsm
+          if is_loc_thread_owned tid location cms then
+            Mreturn cms
           else
-            drop_write_authorisation_of_lock tid addr wmo val pte gsm
+            drop_write_authorisation_of_lock tid addr wmo val pte cms
         end
     end
 .
@@ -502,21 +505,21 @@ Definition drop_write_authorisation
 Definition step_write_aux
   (tid : thread_identifier)
   (wd : trans_write_data)
-  (gsm : ghost_simplified_model) :
-  ghost_simplified_model_result :=
+  (cms : casemate_model_state) :
+  casemate_model_result :=
   let wmo := wd.(twd_mo) in
   let val := wd.(twd_val) in
   let addr := wd.(twd_phys_addr) in
   if negb ((bv_and_64 (phys_addr_val addr) b7) b=? b0)
-    then Merror GSME_unaligned_write else
-  let new_st := drop_write_authorisation tid wd gsm in
+    then Merror CME_unaligned_write else
+  let new_st := drop_write_authorisation tid wd cms in
   let write_update s :=
     match s !! addr with
     | Some (loc) =>
       match loc.(sl_pte) with
       | Some desc =>
         (* If we write to a page table, depending on its state, we update them  *)
-        match desc.(ged_state) with
+        match desc.(eed_state) with
         | SPS_STATE_PTE_VALID av =>
             (step_write_on_valid tid wmo loc val s)
         | SPS_STATE_PTE_INVALID_CLEAN av =>
@@ -524,28 +527,28 @@ Definition step_write_aux
         | SPS_STATE_PTE_INVALID_UNCLEAN av =>
             (step_write_on_invalid_unclean tid wmo loc val s)
         | SPS_STATE_PTE_NOT_WRITABLE =>
-            (Merror (GSME_write_on_not_writable addr))
+            (Merror (CME_write_on_not_writable addr))
         end
       | None => (* If it is not a pte, we just update the value *)
         let new_loc := loc <| sl_val := val |> in
         {|
-          gsmsr_log := nil;
-          gsmsr_data :=
+          cmr_log := nil;
+          cmr_data :=
             Ok _ _ (
-              s <| gsm_memory := <[ addr := new_loc ]> s.(gsm_memory) |>
+              s <| cms_memory := <[ addr := new_loc ]> s.(cms_memory) |>
             );
         |}
       end
     | None =>
       (* If the location has not been written to, it is not a pgt, just save its value *)
-        let new_st := s <| gsm_memory :=
+        let new_st := s <| cms_memory :=
             <[ addr := {|
                 sl_phys_addr := addr;
                 sl_val := val;
                 sl_pte := None;
                 sl_thread_owner := None;
               |}
-            ]> s.(gsm_memory) |> in
+            ]> s.(cms_memory) |> in
                 Mreturn new_st
           end
   in
@@ -555,9 +558,9 @@ Definition step_write_aux
 Function step_write_page
   (tid : thread_identifier)
   (wd : trans_write_data)
-  (res : ghost_simplified_model_result)
+  (res : casemate_model_result)
   (offs : Z) {measure Z.abs_nat offs} :
-  ghost_simplified_model_result :=
+  casemate_model_result :=
   if Zle_bool offs 0 then
     res
   else
@@ -577,74 +580,85 @@ Proof. lia. Qed.
 Definition step_write
   (tid : thread_identifier)
   (wd : trans_write_data)
-  (gsm : ghost_simplified_model) :
-  ghost_simplified_model_result :=
+  (cms : casemate_model_state) :
+  casemate_model_result :=
   match wd.(twd_mo) with
-    | WMO_plain | WMO_release => step_write_aux tid wd gsm
-    | WMO_page => step_write_page tid wd (Mreturn gsm) z512
-end.
+    | WMO_plain | WMO_release => step_write_aux tid wd cms
+    | WMO_page => step_write_page tid wd (Mreturn cms) z512
+  end.
 
 (******************************************************************************************)
-(*                             Code for zalloc                                            *)
+(*                             Code for init                                            *)
 (******************************************************************************************)
 
-Definition step_zalloc_aux
+Definition step_init_aux
   (addr : phys_addr_t)
-  (st : ghost_simplified_model_result) :
-  ghost_simplified_model_result :=
-  let update s := {| gsmsr_log := nil; gsmsr_data := Ok _ _ (s <| gsm_zalloc := <[ addr := () ]> s.(gsm_zalloc) |>) |} in
+  (st : casemate_model_result) :
+  casemate_model_result :=
+  let update s := {| cmr_log := nil; cmr_data := Ok _ _ (s <| cms_initialised := <[ addr := () ]> s.(cms_initialised) |>) |} in
   Mupdate_state update st
 .
 
-Definition _step_zalloc_step_size := Phys_addr (bv_shiftl_64 b1 (bv64.BV64 3)).
+Definition _step_init_step_size := Phys_addr (bv_shiftl_64 b1 (bv64.BV64 3)).
 
-Fixpoint step_zalloc_all
+Fixpoint step_init_all
   (addr : phys_addr_t)
-  (st : ghost_simplified_model_result)
+  (st : casemate_model_result)
   (offs : phys_addr_t)
   (max : nat) :
-  ghost_simplified_model_result :=
+  casemate_model_result :=
   match max with
     | O => st
     | S max =>
-      let st := step_zalloc_aux (addr pa+ offs) st in
-      step_zalloc_all addr st (offs pa+ (_step_zalloc_step_size)) max
+      let st := step_init_aux (addr pa+ offs) st in
+      step_init_all addr st (offs pa+ (_step_init_step_size)) max
   end
 .
 
-Definition step_zalloc
-  (zd : trans_zalloc_data)
-  (gsm : ghost_simplified_model) :
-  ghost_simplified_model_result :=
-  step_zalloc_all (Phys_addr (bv_shiftr_64 (phys_addr_val zd.(tzd_addr)) (bv64.BV64 9))) {|gsmsr_log := nil; gsmsr_data := Ok _ _ gsm|} pa0 (to_nat zd.(tzd_size))
+Definition step_init
+  (init_data : trans_init_data)
+  (cms : casemate_model_state) :
+  casemate_model_result :=
+  step_init_all (Phys_addr (bv_shiftr_64 (phys_addr_val init_data.(tid_addr)) (bv64.BV64 9))) {|cmr_log := nil; cmr_data := Ok _ _ cms|} pa0 (to_nat init_data.(tid_size))
 .
 
 
 (******************************************************************************************)
 (*                             Code for read                                              *)
 (******************************************************************************************)
+Definition step_memset
+  (tid : thread_identifier)
+  (memset_data : trans_memset_data)
+  (cms : casemate_model_state) : casemate_model_result :=
+  let write_data := {|
+    twd_mo := WMO_plain;
+    twd_phys_addr := memset_data.(tmd_addr);
+    twd_val := memset_data.(tmd_value);
+  |} in
+  (* memset is a plain write *)
+  step_write_page tid write_data (Mreturn cms) (bv64.to_Z (bv_shiftr_64 memset_data.(tmd_size) b3)).
 
 Definition step_read
   (tid : thread_identifier)
   (rd : trans_read_data)
-  (gsm : ghost_simplified_model) :
-  ghost_simplified_model_result :=
+  (cms : casemate_model_state) :
+  casemate_model_result :=
   (* Test if the memory has been initialized (it might refuse acceptable executions, not sure if it is a good idea) and its content is consistent. *)
-  match gsm !! rd.(trd_phys_addr) with
+  match cms !! rd.(trd_phys_addr) with
     | Some loc =>
         if loc.(sl_val) b=? rd.(trd_val) then
-          Mreturn gsm
+          Mreturn cms
         else
           let new_loc := loc <| sl_val := rd.(trd_val) |> in
-          {| gsmsr_log :=
+          {| cmr_log :=
               [Inconsistent_read loc.(sl_val) rd.(trd_val) rd.(trd_phys_addr)];
-             gsmsr_data := (Ok _ _ (gsm <| gsm_memory := <[rd.(trd_phys_addr) := new_loc ]> gsm.(gsm_memory) |>)) |}
+             cmr_data := (Ok _ _ (cms <| cms_memory := <[rd.(trd_phys_addr) := new_loc ]> cms.(cms_memory) |>)) |}
     | None =>
         let loc := {| sl_phys_addr := rd.(trd_phys_addr); sl_val := rd.(trd_val); sl_pte := None; sl_thread_owner := Some tid |} in
-        let st := gsm <| gsm_memory := <[ rd.(trd_phys_addr) := loc ]> gsm.(gsm_memory) |> in
-        {| gsmsr_log :=
+        let st := cms <| cms_memory := <[ rd.(trd_phys_addr) := loc ]> cms.(cms_memory) |> in
+        {| cmr_log :=
             [Warning_read_write_non_allocd loc.(sl_phys_addr)];
-           gsmsr_data := Ok _ _ st
+           cmr_data := Ok _ _ st
         |}
   end
 .
@@ -656,26 +670,26 @@ Definition dsb_invalid_unclean_unmark_children
   (cpu_id : thread_identifier)
   (loc : sm_location)
   (lis : aut_invalid_unclean)
-  (ptc : page_table_context) :
-  ghost_simplified_model_result :=
+  (ptc : pgtable_traverse_context) :
+  casemate_model_result :=
   let st := ptc.(ptc_state) in
   let desc := (* This uses the old descriptor to rebuild a fresh old descriptor *)
     deconstruct_pte cpu_id ptc.(ptc_partial_ia) lis.(ai_old_valid_desc) ptc.(ptc_level) ptc.(ptc_root) ptc.(ptc_stage)
   in
-  match desc.(ged_pte_kind) with
+  match desc.(eed_pte_kind) with
     | PTER_PTE_KIND_TABLE map =>
       (* The children are clean, and not writable, otherwise, it would catch fire *)
-      traverse_pgt_from desc.(ged_owner) map.(next_level_table_addr) desc.(ged_ia_region).(range_start) (next_level desc.(ged_level)) desc.(ged_stage) (unmark_cb cpu_id) st
-    | _ => {| gsmsr_log  := nil; gsmsr_data := Ok _ _ st |}
+      traverse_pgt_from desc.(eed_owner) map.(next_level_table_addr) desc.(eed_ia_region).(range_start) (next_level desc.(eed_level)) desc.(eed_stage) (unmark_cb cpu_id) st
+    | _ => {| cmr_log  := nil; cmr_data := Ok _ _ st |}
   end
 .
 
 
 Definition new_pte_after_dsb
   (cpu_id : thread_identifier)
-  (pte : ghost_exploded_descriptor)
-  (kind : DxB) : ghost_exploded_descriptor :=
-  match pte.(ged_state) with
+  (pte : entry_exploded_descriptor)
+  (kind : DxB) : entry_exploded_descriptor :=
+  match pte.(eed_state) with
     | SPS_STATE_PTE_INVALID_UNCLEAN sst =>
       (* DSB has an effect on invalid unclean state only *)
       if negb (bool_decide (sst.(ai_invalidator_tid) = cpu_id)) then
@@ -684,19 +698,19 @@ Definition new_pte_after_dsb
         (* Otherwise, update the state invalid unclean sub-automaton *)
         match sst.(ai_lis) with
           | LIS_unguarded =>
-            pte <|ged_state := SPS_STATE_PTE_INVALID_UNCLEAN (sst <| ai_lis := LIS_dsbed |>) |>
+            pte <|eed_state := SPS_STATE_PTE_INVALID_UNCLEAN (sst <| ai_lis := LIS_dsbed |>) |>
           | LIS_dsbed => pte
           | LIS_dsb_tlbied =>
             match kind.(DxB_domain) with
               | MBReqDomain_InnerShareable | MBReqDomain_FullSystem =>
-                pte <| ged_state := SPS_STATE_PTE_INVALID_CLEAN {| aic_invalidator_tid := sst.(ai_invalidator_tid) |} |>
-                    <| ged_pte_kind := PTER_PTE_KIND_INVALID |>
+                pte <| eed_state := SPS_STATE_PTE_INVALID_CLEAN {| aic_invalidator_tid := sst.(ai_invalidator_tid) |} |>
+                    <| eed_pte_kind := PTER_PTE_KIND_INVALID |>
               | _ => pte
             end
           | LIS_dsb_tlbi_ipa =>
               match kind.(DxB_domain) with
                 | MBReqDomain_InnerShareable | MBReqDomain_FullSystem =>
-                  pte <|ged_state := SPS_STATE_PTE_INVALID_UNCLEAN (sst <|ai_lis := LIS_dsb_tlbi_ipa_dsb |>) |>
+                  pte <|eed_state := SPS_STATE_PTE_INVALID_UNCLEAN (sst <|ai_lis := LIS_dsb_tlbi_ipa_dsb |>) |>
                 | _ => pte
               end
           | _ => pte
@@ -708,21 +722,21 @@ Definition new_pte_after_dsb
 Definition dsb_visitor
   (kind : DxB)
   (cpu_id : thread_identifier)
-  (ctx : page_table_context) :
-  ghost_simplified_model_result :=
+  (ctx : pgtable_traverse_context) :
+  casemate_model_result :=
   match ctx.(ptc_loc) with
     | None => (* This case is not explicitly excluded by the C code, but we cannot do anything in this case. *)
-      Merror (GSME_uninitialised "dsb_visitor"%string ctx.(ptc_addr))
+      Merror (CME_uninitialised "dsb_visitor"%string ctx.(ptc_addr))
     | Some location =>
       match location.(sl_pte) with
-        | None => Merror (GSME_not_a_pte "dsb_visitor" ctx.(ptc_addr))
+        | None => Merror (CME_not_a_pte "dsb_visitor" ctx.(ptc_addr))
         | Some pte =>
           let new_pte := new_pte_after_dsb cpu_id pte kind in
           (* then update state and return *)
           let new_loc := (location <| sl_pte := Some new_pte |>) in
-          let new_state := ctx.(ptc_state) <| gsm_memory := <[ location.(sl_phys_addr) := new_loc ]> ctx.(ptc_state).(gsm_memory) |> in
+          let new_state := ctx.(ptc_state) <| cms_memory := <[ location.(sl_phys_addr) := new_loc ]> ctx.(ptc_state).(cms_memory) |> in
           let log :=
-            match pte.(ged_state), new_pte.(ged_state) with
+            match pte.(eed_state), new_pte.(eed_state) with
               | SPS_STATE_PTE_INVALID_UNCLEAN _ , SPS_STATE_PTE_INVALID_CLEAN _ =>
                 Some (Log "BBM: invalid_unclean->invalid_clean"%string (phys_addr_val location.(sl_phys_addr)))
               | SPS_STATE_PTE_INVALID_UNCLEAN {| ai_lis := LIS_unguarded|} , SPS_STATE_PTE_INVALID_UNCLEAN {| ai_lis := _|} =>
@@ -733,7 +747,7 @@ Definition dsb_visitor
             end
           in
           let new_state :=
-            match pte.(ged_state), new_pte.(ged_state) with
+            match pte.(eed_state), new_pte.(eed_state) with
               | SPS_STATE_PTE_INVALID_UNCLEAN lis , SPS_STATE_PTE_INVALID_CLEAN _ =>
                 dsb_invalid_unclean_unmark_children cpu_id new_loc lis
                     (ctx <| ptc_state := new_state |> <|ptc_loc := Some new_loc|>)
@@ -750,41 +764,41 @@ Definition dsb_visitor
 
 Fixpoint reset_write_authorizations_aux
   (tid : thread_identifier)
-  (roots: list owner_t)
-  (gsm : ghost_simplified_model) :
-  ghost_simplified_model :=
+  (roots: list sm_owner_t)
+  (cms : casemate_model_state) :
+  casemate_model_state :=
   match roots with
-  | [] => gsm
+  | [] => cms
   | h :: q =>
-    match lookup (phys_addr_val (root_val h)) gsm.(gsm_lock_addr) with
+    match lookup (phys_addr_val (root_val h)) cms.(cms_lock_addr) with
     | Some lock_addr =>
       let new_st :=
-        match lookup lock_addr gsm.(gsm_lock_state) with
-        | None => gsm
+        match lookup lock_addr cms.(cms_lock_state) with
+        | None => cms
         | Some thread =>
           if bool_decide (thread = tid) then
-            (gsm <| gsm_lock_authorization := 
-                insert lock_addr write_authorized gsm.(gsm_lock_authorization) |>)
+            (cms <| cms_lock_authorization := 
+                insert lock_addr write_authorized cms.(cms_lock_authorization) |>)
           else
-            gsm
+            cms
         end
       in
       reset_write_authorizations_aux tid q new_st
-    | None => reset_write_authorizations_aux tid q gsm
+    | None => reset_write_authorizations_aux tid q cms
     end
   end
 .
 
 
-Definition reset_write_authorizations (tid : thread_identifier) (gsm : ghost_simplified_model) : ghost_simplified_model :=
+Definition reset_write_authorizations (tid : thread_identifier) (cms : casemate_model_state) : casemate_model_state :=
   (* Reset the authorizations for both states *)
-  reset_write_authorizations_aux tid gsm.(gsm_roots).(pr_s2)
-    (reset_write_authorizations_aux tid gsm.(gsm_roots).(pr_s1) gsm)
+  reset_write_authorizations_aux tid cms.(cms_roots).(cmr_s2)
+    (reset_write_authorizations_aux tid cms.(cms_roots).(cmr_s1) cms)
 .
 
-Definition step_dsb (tid : thread_identifier) (dk : DxB) (gsm : ghost_simplified_model) : ghost_simplified_model_result :=
+Definition step_dsb (tid : thread_identifier) (dk : DxB) (cms : casemate_model_state) : casemate_model_result :=
   (* There is enough barrier now to write plain again *)
-  let st := reset_write_authorizations tid gsm in
+  let st := reset_write_authorizations tid cms in
   (* walk the pgt with dsb_visitor*)
   traverse_all_pgt (Some tid) st (dsb_visitor dk tid)
 .
@@ -807,7 +821,7 @@ Definition is_last_level_only (d : TLBI_op_by_addr_data) : bool :=
   end
 .
 
-Definition should_perform_tlbi (td : TLBI_intermediate) (ptc : page_table_context) : option bool :=
+Definition should_perform_tlbi (td : TLBI_intermediate) (ptc : pgtable_traverse_context) : option bool :=
   match ptc.(ptc_loc) with
     | None => None (* does not happen because we call it in tlbi_visitor in which we test that the location is init *)
     | Some loc =>
@@ -817,13 +831,13 @@ Definition should_perform_tlbi (td : TLBI_intermediate) (ptc : page_table_contex
           match td.(TI_method) with
             | TLBI_by_input_addr d =>
               let tlbi_addr := bv_shiftl_64 (phys_addr_val d.(TOBAD_page)) b12 in
-              let ia_start := pte_desc.(ged_ia_region).(range_start) in
-              let ia_end := ia_start pa+ pte_desc.(ged_ia_region).(range_size) in
-              if (is_leaf pte_desc.(ged_pte_kind)
+              let ia_start := pte_desc.(eed_ia_region).(range_start) in
+              let ia_end := ia_start pa+ pte_desc.(eed_ia_region).(range_size) in
+              if (is_leaf pte_desc.(eed_pte_kind)
                        && (phys_addr_val ia_start b<=? tlbi_addr)
                        && (tlbi_addr b<? phys_addr_val ia_end)) then
                 Some false
-              else if ((negb (is_l3 pte_desc.(ged_level))) && is_last_level_only d) then
+              else if ((negb (is_l3 pte_desc.(eed_level))) && is_last_level_only d) then
                 Some false
               else
                 Some true
@@ -862,23 +876,23 @@ Definition step_pte_on_tlbi_after_tlbi_ipa (td: TLBI_intermediate) : option LIS 
 Definition tlbi_visitor
   (cpu_id : thread_identifier)
   (td : TLBI_intermediate)
-  (ptc : page_table_context) : 
-  ghost_simplified_model_result :=
+  (ptc : pgtable_traverse_context) : 
+  casemate_model_result :=
   match ptc.(ptc_loc) with
     | None => (* Cannot do anything if the page is not initialized *)
-      Merror (GSME_uninitialised "tlbi_visitor" ptc.(ptc_addr))
+      Merror (CME_uninitialised "tlbi_visitor" ptc.(ptc_addr))
     | Some location =>
       (* Test if there is something to do *)
       match should_perform_tlbi td ptc with
-        | None => Merror GSME_unimplemented
+        | None => Merror CME_unimplemented
         | Some b =>
           if b then
             (* step_pte_on_tlbi: inlined *)
             match location.(sl_pte) with
-              | None => Merror (GSME_internal_error IET_unexpected_none)
+              | None => Merror (CME_internal_error IET_unexpected_none)
                 (* This cannot happen (otherwise, should_perform_tlbi would be false) *)
               | Some exploded_desc =>
-                match exploded_desc.(ged_state) with
+                match exploded_desc.(eed_state) with
                   | SPS_STATE_PTE_INVALID_UNCLEAN ai =>
                     (* If the CPU that does the transformation is not the one that initiated the invalidation, do nothing *)
                     if bool_decide (cpu_id = ai.(ai_invalidator_tid)) then
@@ -891,7 +905,7 @@ Definition tlbi_visitor
                         end
                       in
                       match new_substate with
-                        | None => Merror GSME_unimplemented
+                        | None => Merror CME_unimplemented
                         | Some new_substate =>
                           let log :=
                             match new_substate, ai.(ai_lis) with
@@ -902,8 +916,8 @@ Definition tlbi_visitor
                             end
                           in
                           (* Write the new sub-state in the global automaton *)
-                          let new_loc := location <| sl_pte := Some (exploded_desc <|ged_state := SPS_STATE_PTE_INVALID_UNCLEAN (ai <| ai_lis := new_substate|>) |>)|> in
-                          let new_mem := ptc.(ptc_state) <| gsm_memory := <[location.(sl_phys_addr) := new_loc]> ptc.(ptc_state).(gsm_memory)|> in
+                          let new_loc := location <| sl_pte := Some (exploded_desc <|eed_state := SPS_STATE_PTE_INVALID_UNCLEAN (ai <| ai_lis := new_substate|>) |>)|> in
+                          let new_mem := ptc.(ptc_state) <| cms_memory := <[location.(sl_phys_addr) := new_loc]> ptc.(ptc_state).(cms_memory)|> in
                           log (Mreturn new_mem)
                       end
                     else
@@ -912,26 +926,26 @@ Definition tlbi_visitor
                 end
             end
           else (* In the case where the PTE is not affected by the TLBI, we do nothing *)
-            {|gsmsr_log := nil; gsmsr_data := Ok _ _ ptc.(ptc_state) |}
+            {|cmr_log := nil; cmr_data := Ok _ _ ptc.(ptc_state) |}
       end
   end
 .
 
-Definition step_tlbi (tid : thread_identifier) (td : TLBI) (gsm : ghost_simplified_model) : ghost_simplified_model_result :=
+Definition step_tlbi (tid : thread_identifier) (td : TLBI) (cms : casemate_model_state) : casemate_model_result :=
   match decode_tlbi td with
-  | None => Merror GSME_unimplemented
+  | None => Merror CME_unimplemented
   | Some decoded_TLBI =>
     match td.(TLBI_rec).(TLBIRecord_regime) with
     | Regime_EL2 =>
       (* traverse all s1 pages*)
-      traverse_si_pgt (Some tid) gsm (tlbi_visitor tid decoded_TLBI) S1
+      traverse_si_pgt (Some tid) cms (tlbi_visitor tid decoded_TLBI) S1
     | Regime_EL10 =>
       (* traverse s2 pages *)
-      traverse_si_pgt (Some tid) gsm (tlbi_visitor tid decoded_TLBI) S2
+      traverse_si_pgt (Some tid) cms (tlbi_visitor tid decoded_TLBI) S2
     | _ =>
       (* traverse all page tables and add a warning *)
-      let res := traverse_all_pgt (Some tid) gsm (tlbi_visitor tid decoded_TLBI) in
-      res <| gsmsr_log := Warning_unsupported_TLBI :: res.(gsmsr_log) |>
+      let res := traverse_all_pgt (Some tid) cms (tlbi_visitor tid decoded_TLBI) in
+      res <| cmr_log := Warning_unsupported_TLBI :: res.(cmr_log) |>
     end
   end
 .
@@ -941,7 +955,7 @@ Definition step_tlbi (tid : thread_identifier) (td : TLBI) (gsm : ghost_simplifi
 (*                                  Step MSR                                              *)
 (******************************************************************************************)
 
-Fixpoint si_root_exists (root : owner_t) (roots : list owner_t) : bool :=
+Fixpoint si_root_exists (root : sm_owner_t) (roots : list sm_owner_t) : bool :=
   match roots with
     | [] => false
     | t :: q => (bool_decide (t = root)) || (si_root_exists root q)
@@ -949,40 +963,40 @@ Fixpoint si_root_exists (root : owner_t) (roots : list owner_t) : bool :=
 .
 
 Definition _extract_si_root_big_bv := BV64 0xfffffffffffe%Z. (* GENMASK (b47) (b1) *)
-Definition extract_si_root (val : u64) (stage : stage_t) : owner_t :=
+Definition extract_si_root (val : u64) (stage : entry_stage_t) : sm_owner_t :=
   (* Does not depends on the S1/S2 level but two separate functions in C, might depend on CPU config *)
   Root (Phys_addr (bv_and_64 val _extract_si_root_big_bv))
 .
 
 Definition register_si_root
   (tid : thread_identifier)
-  (gsm : ghost_simplified_model) 
-  (root : owner_t)
-  (stage : stage_t) : 
-  ghost_simplified_model_result :=
+  (cms : casemate_model_state) 
+  (root : sm_owner_t)
+  (stage : entry_stage_t) : 
+  casemate_model_result :=
   let other_root_list :=
     match stage with
-      | S1 => pr_s2
-      | S2 => pr_s1
-    end gsm.(gsm_roots) in
+      | S1 => cmr_s2
+      | S2 => cmr_s1
+    end cms.(cms_roots) in
   (* Check that the root does not already exist in the other root list*)
-  if si_root_exists root other_root_list then Merror GSME_root_already_exists  
+  if si_root_exists root other_root_list then Merror CME_root_already_exists  
   else
     (* Add the root to the list of roots*)
     let new_roots :=
       match stage with
-        | S2 => gsm.(gsm_roots) <| pr_s2 := root :: gsm.(gsm_roots).(pr_s2) |>
-        | S1 => gsm.(gsm_roots) <| pr_s1 := root :: gsm.(gsm_roots).(pr_s1) |>
+        | S2 => cms.(cms_roots) <| cmr_s2 := root :: cms.(cms_roots).(cmr_s2) |>
+        | S1 => cms.(cms_roots) <| cmr_s1 := root :: cms.(cms_roots).(cmr_s1) |>
       end
     in
-    let new_st := gsm <| gsm_roots := new_roots |> in
+    let new_st := cms <| cms_roots := new_roots |> in
     (* then mark all its children as PTE *)
     match root with
       | Root r => traverse_pgt_from root r pa0 l0 stage (mark_cb tid) new_st
     end
 .
 
-Definition step_msr (tid : thread_identifier) (md : trans_msr_data) (gsm : ghost_simplified_model) : ghost_simplified_model_result :=
+Definition step_msr (tid : thread_identifier) (md : trans_msr_data) (cms : casemate_model_state) : casemate_model_result :=
   let stage :=
     match md.(tmd_sysreg) with
       | SYSREG_TTBR_EL2 => S1
@@ -993,15 +1007,15 @@ Definition step_msr (tid : thread_identifier) (md : trans_msr_data) (gsm : ghost
   (* The value written to TTRB is a root, it might be new. *)
   let roots :=
     match stage with
-      | S2 =>  pr_s2
-      | S1 => pr_s1
-    end gsm.(gsm_roots)
+      | S2 =>  cmr_s2
+      | S1 => cmr_s1
+    end cms.(cms_roots)
   in
-  if si_root_exists root (match stage with | S2 =>  pr_s2 | S1 => pr_s1 end gsm.(gsm_roots)) then
-    Mreturn gsm (* If it is already known to be a root, do nothing, it has already been registered *)
+  if si_root_exists root (match stage with | S2 =>  cmr_s2 | S1 => cmr_s1 end cms.(cms_roots)) then
+    Mreturn cms (* If it is already known to be a root, do nothing, it has already been registered *)
   else
     (* Otherwise, register it *)
-    register_si_root tid gsm root stage
+    register_si_root tid cms root stage
 .
 
 (******************************************************************************************)
@@ -1009,42 +1023,42 @@ Definition step_msr (tid : thread_identifier) (md : trans_msr_data) (gsm : ghost
 (******************************************************************************************)
 
 Definition step_hint_set_root_lock
-  (root : owner_t)
+  (root : sm_owner_t)
   (addr : phys_addr_t)
-  (gsm : ghost_simplified_model) :
-  ghost_simplified_model_result :=
-    Mreturn (gsm <| gsm_lock_addr := insert (phys_addr_val (root_val root)) (phys_addr_val addr) gsm.(gsm_lock_addr)|>)
+  (cms : casemate_model_state) :
+  casemate_model_result :=
+    Mreturn (cms <| cms_lock_addr := insert (phys_addr_val (root_val root)) (phys_addr_val addr) cms.(cms_lock_addr)|>)
 .
 
 Function set_owner_root
   (phys : phys_addr_t)
-  (root : owner_t)
-  (gsm : ghost_simplified_model)
+  (root : sm_owner_t)
+  (cms : casemate_model_state)
   (logs : list log_element)
   (offs : Z) 
   {measure Z.abs_nat offs} : 
-  ghost_simplified_model_result :=
+  casemate_model_result :=
   if Zle_bool offs 0 then
-    {| gsmsr_log := logs; gsmsr_data := Ok _ _ gsm |}
+    {| cmr_log := logs; cmr_data := Ok _ _ cms |}
   else
     let addr := phys pa+ (Phys_addr (bv_mul_Z_64 b8 (offs - 1))) in
-    match gsm !! addr with
+    match cms !! addr with
       | None =>
         {|
-          gsmsr_log :=
+          cmr_log :=
             logs;
-            gsmsr_data := Error _ _ (GSME_uninitialised "set_owner_root" addr)
+            cmr_data := Error _ _ (CME_uninitialised "set_owner_root" addr)
         |}
       | Some location =>
         let new_pte :=
           match location.(sl_pte) with
             | None => None
-            | Some pte => Some (pte <| ged_owner := root|>) (* actually change the root *)
+            | Some pte => Some (pte <| eed_owner := root|>) (* actually change the root *)
           end
         in
         (* Write the change to the global state *)
         let new_loc := location <| sl_pte := new_pte |> in
-        let new_state := gsm <|gsm_memory := <[ location.(sl_phys_addr) := new_loc ]> gsm.(gsm_memory) |> in
+        let new_state := cms <|cms_memory := <[ location.(sl_phys_addr) := new_loc ]> cms.(cms_memory) |> in
         set_owner_root phys root new_state logs (offs - 1)
     end
 .
@@ -1052,16 +1066,16 @@ Set Warnings "-funind-cannot-build-inversion -funind-cannot-define-graph".
 Proof. lia. Qed.
 Set Warnings "funind-cannot-build-inversion funind-cannot-define-graph".
 
-Definition step_release_cb (ctx : page_table_context) : ghost_simplified_model_result :=
+Definition step_release_cb (ctx : pgtable_traverse_context) : casemate_model_result :=
     match ctx.(ptc_loc) with
-    | None => Merror (GSME_uninitialised "step_release_cb"%string ctx.(ptc_addr))
+    | None => Merror (CME_uninitialised "step_release_cb"%string ctx.(ptc_addr))
     | Some location =>
       match location.(sl_pte) with
-        | None => Merror (GSME_not_a_pte "release_cb" ctx.(ptc_addr))
+        | None => Merror (CME_not_a_pte "release_cb" ctx.(ptc_addr))
         | Some desc =>
-          match desc.(ged_state) with
+          match desc.(eed_state) with
             | SPS_STATE_PTE_INVALID_UNCLEAN _ =>
-                Merror (GSME_bbm_violation VT_release_unclean ctx.(ptc_addr))
+                Merror (CME_bbm_violation VT_release_unclean ctx.(ptc_addr))
             | _ => Mreturn ctx.(ptc_state)
           end
       end
@@ -1069,7 +1083,7 @@ Definition step_release_cb (ctx : page_table_context) : ghost_simplified_model_r
 .
 
 
-Fixpoint remove (x : owner_t) (l : list owner_t) : list owner_t :=
+Fixpoint remove (x : sm_owner_t) (l : list sm_owner_t) : list sm_owner_t :=
   match l with
     | nil => nil
     | y::tl => if bool_decide (x = y) then remove x tl else y::(remove x tl)
@@ -1077,47 +1091,47 @@ Fixpoint remove (x : owner_t) (l : list owner_t) : list owner_t :=
 .
 
 Definition try_unregister_root
-  (addr : owner_t)
+  (addr : sm_owner_t)
   (cpu : thread_identifier)
-  (gsm : ghost_simplified_model) :
-  ghost_simplified_model_result :=
-  match gsm !! root_val addr with
-    | None => Merror (GSME_internal_error IET_unexpected_none)
+  (cms : casemate_model_state) :
+  casemate_model_result :=
+  match cms !! root_val addr with
+    | None => Merror (CME_internal_error IET_unexpected_none)
     | Some loc =>
       match loc.(sl_pte) with
-        | None => Merror (GSME_internal_error IET_unexpected_none)
+        | None => Merror (CME_internal_error IET_unexpected_none)
         | Some pte =>
           let new_roots :=
-            match pte.(ged_stage) with
-              | S2 => gsm.(gsm_roots) <| pr_s2 := remove addr gsm.(gsm_roots).(pr_s2) |>
-              | S1 => gsm.(gsm_roots) <| pr_s1 := remove addr gsm.(gsm_roots).(pr_s1) |>
+            match pte.(eed_stage) with
+              | S2 => cms.(cms_roots) <| cmr_s2 := remove addr cms.(cms_roots).(cmr_s2) |>
+              | S1 => cms.(cms_roots) <| cmr_s1 := remove addr cms.(cms_roots).(cmr_s1) |>
             end
           in
-          let gsm := gsm <| gsm_roots := new_roots |> in
-          traverse_pgt_from_root addr pte.(ged_stage) (unmark_cb cpu) gsm
+          let cms := cms <| cms_roots := new_roots |> in
+          traverse_pgt_from_root addr pte.(eed_stage) (unmark_cb cpu) cms
       end
   end
 .
 
 Definition step_release_table
   (cpu : thread_identifier)
-  (addr : owner_t)
-  (gsm : ghost_simplified_model) : 
-  ghost_simplified_model_result :=
-  match gsm !! root_val addr with
-    | None => Merror (GSME_uninitialised "release"%string (root_val addr))
+  (addr : sm_owner_t)
+  (cms : casemate_model_state) : 
+  casemate_model_result :=
+  match cms !! root_val addr with
+    | None => Merror (CME_uninitialised "release"%string (root_val addr))
     | Some location =>
       match location.(sl_pte) with
-        | None => Merror (GSME_not_a_pte "release"%string (root_val addr))
+        | None => Merror (CME_not_a_pte "release"%string (root_val addr))
         | Some desc =>
           let new_st := traverse_pgt_from
             addr
-            (root_val desc.(ged_owner))
-            desc.(ged_ia_region).(range_start)
-            desc.(ged_level)
-            desc.(ged_stage)
+            (root_val desc.(eed_owner))
+            desc.(eed_ia_region).(range_start)
+            desc.(eed_level)
+            desc.(eed_stage)
             step_release_cb
-            gsm in
+            cms in
           Mupdate_state (try_unregister_root (addr) cpu) new_st
       end
   end
@@ -1125,18 +1139,18 @@ Definition step_release_table
 
 Definition step_hint_set_pte_thread_owner
   (phys : phys_addr_t)
-  (val : owner_t)
-  (gsm : ghost_simplified_model) :
-  ghost_simplified_model_result := 
-  match gsm !! phys with
-    | None => Merror (GSME_uninitialised "set_pte_thread_owner"%string phys)
+  (val : sm_owner_t)
+  (cms : casemate_model_state) :
+  casemate_model_result := 
+  match cms !! phys with
+    | None => Merror (CME_uninitialised "set_pte_thread_owner"%string phys)
     | Some location =>
       match location.(sl_pte) with
-        | None => Merror (GSME_not_a_pte "set_pte_thread_owner"%string phys)
+        | None => Merror (CME_not_a_pte "set_pte_thread_owner"%string phys)
         | Some _ =>
           let thread_owner := Thread_identifier (to_nat (phys_addr_val (root_val val))) in
-          Mreturn (gsm <| gsm_memory :=
-            (<[ location.(sl_phys_addr) := location <| sl_thread_owner := Some thread_owner |> ]> gsm.(gsm_memory))
+          Mreturn (cms <| cms_memory :=
+            (<[ location.(sl_phys_addr) := location <| sl_thread_owner := Some thread_owner |> ]> cms.(cms_memory))
           |> )
       end
   end
@@ -1145,22 +1159,22 @@ Definition step_hint_set_pte_thread_owner
 Definition step_hint
   (cpu : thread_identifier)
   (hd : trans_hint_data)
-  (gsm : ghost_simplified_model)
-: ghost_simplified_model_result :=
+  (cms : casemate_model_state)
+: casemate_model_result :=
   match hd.(thd_hint_kind) with
     | GHOST_HINT_SET_ROOT_LOCK =>
       (* The types are weird here because of the order is reversed from SET_OWNER_ROOT (the root is first and the address second) *)
-      step_hint_set_root_lock (Root hd.(thd_location)) (root_val hd.(thd_value)) gsm
+      step_hint_set_root_lock (Root hd.(thd_location)) (root_val hd.(thd_value)) cms
       (* AFAIK, this only affects the internal locking discipline of the C casemate model and does nothing on the Coq version *)
     | GHOST_HINT_SET_OWNER_ROOT =>
       (* When ownership is transferred *)
       (* Not sure about the size of the iteration *)
-      set_owner_root (align_4k hd.(thd_location)) hd.(thd_value) gsm [] z512
-    | GHOST_HINT_RELEASE =>
-      step_release_table cpu (Root hd.(thd_location)) gsm
+      set_owner_root (align_4k hd.(thd_location)) hd.(thd_value) cms [] z512
+    | GHOST_HINT_RELEASE_TABLE =>
+      step_release_table cpu (Root hd.(thd_location)) cms
     | GHOST_HINT_SET_PTE_THREAD_OWNER =>
       (* Set an owner thread of the PTE to track private ownership *)
-      step_hint_set_pte_thread_owner hd.(thd_location) hd.(thd_value) gsm
+      step_hint_set_pte_thread_owner hd.(thd_location) hd.(thd_value) cms
   end
 .
 
@@ -1171,20 +1185,57 @@ Definition step_hint
 
 Definition step_lock
   (cpu : thread_identifier)
-  (hd : trans_lock_data)
-  (gsm : ghost_simplified_model)
-: ghost_simplified_model_result :=
-  match hd.(tld_kind), lookup (phys_addr_val hd.(tld_addr)) gsm.(gsm_lock_state) with
-    | LOCK, None =>(* lock and authorize to write to that page-table *)
-        Mreturn (gsm <| gsm_lock_state := insert (phys_addr_val hd.(tld_addr)) cpu gsm.(gsm_lock_state) |>
-                    <| gsm_lock_authorization := insert (phys_addr_val hd.(tld_addr)) write_authorized gsm.(gsm_lock_authorization)|>)
-    | UNLOCK, Some thread =>
-      if bool_decide (thread = cpu) then
-        Mreturn (gsm <| gsm_lock_state := delete (phys_addr_val hd.(tld_addr)) gsm.(gsm_lock_state) |>)
-      else
-        Merror (GSME_double_lock_acquire cpu thread)
-    | LOCK, Some thread => Merror (GSME_double_lock_acquire cpu thread)
-    | UNLOCK, None => Merror (GSME_double_lock_acquire cpu cpu)
+  (lock_data : trans_lock_data)
+  (cms : casemate_model_state)
+: casemate_model_result :=
+  match lookup (phys_addr_val lock_data.(tld_addr)) cms.(cms_lock_state) with
+  | None =>(* lock and authorize to write to that page-table *)
+      Mreturn (cms <| cms_lock_state := insert (phys_addr_val lock_data.(tld_addr)) cpu cms.(cms_lock_state) |>
+                  <| cms_lock_authorization := insert (phys_addr_val lock_data.(tld_addr)) write_authorized cms.(cms_lock_authorization)|>)
+  | Some thread => Merror (CME_double_lock_acquire cpu thread)
   end
 .
 
+Definition step_unlock
+  (cpu : thread_identifier)
+  (lock_data : trans_lock_data)
+  (cms : casemate_model_state)
+: casemate_model_result :=
+  match lookup (phys_addr_val lock_data.(tld_addr)) cms.(cms_lock_state) with
+  | Some thread =>
+    if bool_decide (thread = cpu) then
+      Mreturn (cms <| cms_lock_state := delete (phys_addr_val lock_data.(tld_addr)) cms.(cms_lock_state) |>)
+    else
+      Merror (CME_double_lock_acquire cpu thread)
+  | None => Merror (CME_double_lock_acquire cpu cpu)
+  end
+.
+
+Definition step
+  (trans : casemate_model_step)
+  (cms : casemate_model_state) :
+  casemate_model_result :=
+  match trans.(cms_data) with
+  | CMSD_TRANS_HW_MEM_WRITE wd =>
+    step_write trans.(cms_thread_identifier) wd cms
+  | CMSD_TRANS_HW_MEM_READ rd =>
+    step_read trans.(cms_thread_identifier) rd cms
+  | CMSD_TRANS_HW_BARRIER (Barrier_DSB dsb_data) =>
+    step_dsb trans.(cms_thread_identifier) dsb_data cms
+  | CMSD_TRANS_HW_BARRIER (_) =>
+    {| cmr_log := []; cmr_data := Ok _ _ cms |}
+  | CMSD_TRANS_HW_TLBI tlbi_data =>
+    step_tlbi trans.(cms_thread_identifier) tlbi_data cms
+  | CMSD_TRANS_HW_MSR msr_data =>
+    step_msr trans.(cms_thread_identifier) msr_data cms
+  | CMSD_TRANS_ABS_LOCK lock_data =>
+    step_lock trans.(cms_thread_identifier) lock_data cms
+  | CMSD_TRANS_ABS_UNLOCK lock_data =>
+    step_unlock trans.(cms_thread_identifier) lock_data cms
+  | CMSD_TRANS_ABS_MEM_INIT init_data =>
+    step_init init_data cms
+  | CMSD_TRANS_ABS_MEMSET memset_data =>
+    step_memset trans.(cms_thread_identifier) memset_data cms
+  | CMSD_TRANS_HINT hint_data =>
+    step_hint trans.(cms_thread_identifier) hint_data cms
+  end.
